backend/Debugvarproof.v
@@ -424,17 +424,13 @@ Proof.
 - (* load *)
   econstructor; split.
   eapply plus_left.
-  eapply exec_Lload with (a := a).
-  rewrite <- H; apply eval_addressing_preserved; exact symbols_preserved.
-  eauto. eauto.
+  eapply exec_Lload with (a := a); eauto.
   apply eval_add_delta_ranges. traceEq.
   constructor; auto.
 - (* store *)
   econstructor; split.
   eapply plus_left.
-  eapply exec_Lstore with (a := a).
-  rewrite <- H; apply eval_addressing_preserved; exact symbols_preserved.
-  eauto. eauto.
+  eapply exec_Lstore with (a := a); eauto.
   apply eval_add_delta_ranges. traceEq.
   constructor; auto.
 - (* call *)
